day1/eval.fst
@@ -1,0 +1,30 @@
+module Eval
+
+open Try
+open Ast
+
+val get : nat -> env -> result (vterm value)
+let rec get i env =
+    match i, env with
+    | 0, e::_ -> return e
+    | i, _::t -> get (i-1) t
+    | _, _ -> throwError "Not found"
+
+val vapply : vterm value -> vterm value -> Dv (result (vterm value))
+
+let rec eval e d =
+    match e with
+    | Annoted e _ -> eval e d
+    | Bound j     -> get j d
+    | Free x      -> return (VNeutral (NFree x))
+    | Apply e1 e2 -> (match eval e1 d, eval e2 d with
+                     | Success v1, Success v2 -> vapply v1 v2
+                     | Failure f, _           -> throwError f
+                     | _, Failure f           -> throwError f)
+    | Inferable e -> eval e d
+    | Lambda e    -> return (VClosure e d)
+
+and vapply e v =
+    match e with 
+    | VClosure e d -> eval e (v::d)
+    | VNeutral n   -> return (VNeutral (NApp n v))
