day1/try.fsti
@@ -6,13 +6,13 @@ type result a  : Type =
     | Success  : a -> result a
     | Failure  : string -> result a
 
-val return     : #a:Type -> a -> Tot (result a)
-val throwError : #a:Type -> string -> Tot (result a)
+val return     : #a:Type -> a -> result a
+val throwError : #a:Type -> string -> result a
 
 val fold       : #a:Type -> #b:Type -> result a -> (a -> b) -> (string -> b) -> b
-val (<$>)      : #a:Type -> #b:Type -> (a -> b) -> result a -> Tot (result b)
-val (<*>)      : #a:Type -> #b:Type -> result (a -> b) -> result a -> Tot (result b)
-val join       : #a:Type -> result (result a) -> Tot (result a)
-val (>>=)      : #a:Type -> #b:Type -> result a -> (a -> result b) -> Tot (result b)
-val unless     : #a:Type -> result a -> (a -> bool) -> result a -> Tot (result a)
+val (<$>)      : #a:Type -> #b:Type -> (a -> b) -> result a -> result b
+val (<*>)      : #a:Type -> #b:Type -> result (a -> b) -> result a -> result b
+val join       : #a:Type -> result (result a) -> result a
+val (>>=)      : #a:Type -> #b:Type -> result a -> (a -> result b) -> result b
+val unless     : #a:Type -> result a -> (a -> bool) -> result a -> result a
 
